WP1-Programming-Languages-Semantics/WP11-C-semantics/src/IMP-Lenses/utp/utp_hoare.thy
@@ -6,38 +6,79 @@ begin
 
 named_theorems hoare
 
+subsection {*Hoare triple definition*}
+
+text {*A Hoare triple is represented by a pre-condition @{text P} a post-condition @{text Q}
+       and a program @{text C}. It says whenever the pre-condition @{text P} holds on the initial state
+       then the post-condition @{text Q} must hold on the final state and this 
+       after the execution of the program @{text C}.*}
+
 definition hoare_r :: "'\<alpha> cond \<Rightarrow> '\<alpha> hrel \<Rightarrow> '\<alpha> cond \<Rightarrow> bool" ("\<lbrace>_\<rbrace>_\<lbrace>_\<rbrace>\<^sub>u") where
 "\<lbrace>p\<rbrace>Q\<lbrace>r\<rbrace>\<^sub>u = ((\<lceil>p\<rceil>\<^sub>< \<Rightarrow> \<lceil>r\<rceil>\<^sub>>) \<sqsubseteq> Q)"
 
 declare hoare_r_def [upred_defs]
 
-lemma hoare_r_conj [hoare]: 
-  assumes"\<lbrace>p\<rbrace>Q\<lbrace>r\<rbrace>\<^sub>u" and "\<lbrace>p\<rbrace>Q\<lbrace>s\<rbrace>\<^sub>u"  
-  shows "\<lbrace>p\<rbrace>Q\<lbrace>r \<and> s\<rbrace>\<^sub>u"
-  by (insert assms) rel_auto
+lemma hoare_true [hoare]: "\<lbrace>P\<rbrace>C\<lbrace>true\<rbrace>\<^sub>u"
+  by rel_auto
+
+lemma hoare_false [hoare]: "\<lbrace>false\<rbrace>C\<lbrace>Q\<rbrace>\<^sub>u"
+  by rel_auto
+
+subsection {*Hoare for Consequence*}
 
 lemma hoare_r_conseq [hoare]: 
   assumes "`p\<^sub>1 \<Rightarrow> p\<^sub>2`" and "\<lbrace>p\<^sub>2\<rbrace>S\<lbrace>q\<^sub>2\<rbrace>\<^sub>u" and "`q\<^sub>2 \<Rightarrow> q\<^sub>1`" 
   shows   "\<lbrace>p\<^sub>1\<rbrace>S\<lbrace>q\<^sub>1\<rbrace>\<^sub>u"
   by (insert assms) rel_auto
 
+subsection {*Precondition strengthening*}
+
+lemma hoare_pre_str[hoare]:
+  assumes "`p\<^sub>1 \<Rightarrow> p\<^sub>2`" and "\<lbrace>p\<^sub>2\<rbrace>C\<lbrace>Q\<rbrace>\<^sub>u"
+  shows "\<lbrace>p\<^sub>1\<rbrace>C\<lbrace>Q\<rbrace>\<^sub>u" 
+  by (insert assms) rel_auto
+
+subsection {*Post-condition weakening*}
+
+lemma hoare_post_weak[hoare]:
+  assumes 1:"\<lbrace>P\<rbrace>C\<lbrace>Q\<^sub>2\<rbrace>\<^sub>u"  
+  and     2:"`Q\<^sub>2 \<Rightarrow> Q\<^sub>1`"
+  shows "\<lbrace>P\<rbrace>C\<lbrace>Q\<^sub>1\<rbrace>\<^sub>u" 
+ by (insert assms) rel_auto
+
+subsection {*Hoare and assertion logic*}
+
+lemma hoare_r_conj [hoare]: 
+  assumes"\<lbrace>p\<rbrace>Q\<lbrace>r\<rbrace>\<^sub>u" and "\<lbrace>p\<rbrace>Q\<lbrace>s\<rbrace>\<^sub>u"  
+  shows "\<lbrace>p\<rbrace>Q\<lbrace>r \<and> s\<rbrace>\<^sub>u"
+  by (insert assms) rel_auto
+subsection {*Hoare SKIP*}
+
+lemma skip_hoare_r [hoare]: "\<lbrace>p\<rbrace>SKIP\<lbrace>p\<rbrace>\<^sub>u"
+  by rel_auto
+
+subsection {*Hoare for assignment*}
+
 lemma assigns_hoare_r [hoare]: 
   assumes"`p \<Rightarrow> \<sigma> \<dagger> q`" 
   shows  "\<lbrace>p\<rbrace>\<langle>\<sigma>\<rangle>\<^sub>a\<lbrace>q\<rbrace>\<^sub>u"
   by (insert assms) rel_auto
 
-lemma skip_hoare_r [hoare]: "\<lbrace>p\<rbrace>SKIP\<lbrace>p\<rbrace>\<^sub>u"
-  by rel_auto
+subsection {*Hoare for Sequential Composition*}
 
 lemma seq_hoare_r [hoare]: 
   assumes"\<lbrace>p\<rbrace>Q\<^sub>1\<lbrace>s\<rbrace>\<^sub>u" and "\<lbrace>s\<rbrace>Q\<^sub>2\<lbrace>r\<rbrace>\<^sub>u" 
   shows"\<lbrace>p\<rbrace>Q\<^sub>1 ;; Q\<^sub>2\<lbrace>r\<rbrace>\<^sub>u"
   by (insert assms) rel_auto
 
+subsection {*Hoare for Conditional*}
+
 lemma cond_hoare_r [hoare]: 
   assumes "\<lbrace>b \<and> p\<rbrace>S\<lbrace>q\<rbrace>\<^sub>u" and "\<lbrace>\<not>b \<and> p\<rbrace>T\<lbrace>q\<rbrace>\<^sub>u" 
   shows "\<lbrace>p\<rbrace>S \<triangleleft> b \<triangleright>\<^sub>r T\<lbrace>q\<rbrace>\<^sub>u"
   by (insert assms) rel_auto
+
+subsection {*Hoare for While-loop*}
 
 lemma while_hoare_r [hoare]:
   assumes "\<lbrace>p \<and> b\<rbrace>S\<lbrace>p\<rbrace>\<^sub>u"
